formula_theory.v
@@ -1,66 +1,58 @@
 Module FormulaTheory.
 Require Export form name decidability feature_model.
 Import Name Form Decidability FeatureModel.
-Require Export Coq.Lists.ListSet.
-Require Export Coq.Lists.List.
-Require Export Coq.Bool.Bool.
-Require Export Coq.Classes.RelationClasses.
+Require Import Coq.Lists.ListSet Coq.Lists.List.
 
 (*yields names for a formula*)
-Fixpoint names (f : Formula) : set Name :=
+Fixpoint names_ (f : Formula) : set Name :=
   match f with
-    | TRUE_FORMULA => empty_set Name
-    | FALSE_FORMULA => empty_set Name
+    | TRUE_FORMULA    => empty_set Name
+    | FALSE_FORMULA   => empty_set Name
     | NAME_FORMULA n1 => set_add name_dec n1 nil
-    | NOT_FORMULA f1 => names f1
-    | AND_FORMULA f1 f2 => set_union name_dec  (names f1) (set_diff name_dec  (names f2) (names f1))  
-    | IMPLIES_FORMULA f1 f2 => set_union name_dec  (names f1) (set_diff name_dec  (names f2) (names f1)) 
-  end.
+    | NOT_FORMULA f1  => names_ f1
+    | AND_FORMULA f1 f2     => set_union name_dec  (names_ f1) 
+                                  (set_diff name_dec  (names_ f2) (names_ f1))  
+    | IMPLIES_FORMULA f1 f2 => set_union name_dec  (names_ f1) 
+                                  (set_diff name_dec  (names_ f2) (names_ f1)) 
+  end.  
+
 
 (* indicates whether a formula is well-typed*)
-Fixpoint wt (fs : features) (f : Formula) : Prop :=
+Fixpoint wt (fm : FM) (f : Formula) : Prop :=
   match f with
-    | TRUE_FORMULA => True
-    | FALSE_FORMULA => True
-    | NAME_FORMULA n1 => In n1 fs
-    | NOT_FORMULA f1 => wt fs f1
-    | AND_FORMULA f1 f2 => (wt fs f1) /\ (wt fs f2)  
-    | IMPLIES_FORMULA f1 f2 => (wt fs f1) /\ (wt fs f2)
+    | TRUE_FORMULA    => True
+    | FALSE_FORMULA   => True
+    | NAME_FORMULA n1 => set_In n1 (fst fm)
+    | NOT_FORMULA f1  => wt fm f1
+    | AND_FORMULA f1 f2     => (wt fm f1) /\ (wt fm f2)  
+    | IMPLIES_FORMULA f1 f2 => (wt fm f1) /\ (wt fm f2)
    end.
 
-Fixpoint wtFormulaeAux(fm : FM) (fs : formulae): Prop :=
-   match fs with 
-     | nil => True
-     | a1 :: x1 => (wt (names_ fm) a1) /\ (wtFormulaeAux fm x1)
-   end.
- 
 (*indicates whether a feature model has all of its formulae well-typed*)
-Fixpoint wtFormulae (fm : FM) : Prop := 
-  wtFormulaeAux fm (formulas fm).
+Definition wfFormulae (fm: FM) : Prop :=
+  forall (f: Formula), set_In f (formulas fm) -> wt fm f.
 
 (*indicates when a configuration satisfies a formula*)
 Fixpoint satisfies (f: Formula) ( c : Configuration) : Prop :=
   match f with
-    | TRUE_FORMULA => True
-    | FALSE_FORMULA => False
+    | TRUE_FORMULA   => True
+    | FALSE_FORMULA  => False
     | NAME_FORMULA n => set_In n c
-    | NOT_FORMULA f1 => ~(satisfies f1 c)
-    | AND_FORMULA f1 f2 => (satisfies f1 c) /\ (satisfies f2 c)  
+    | NOT_FORMULA f1 => not (satisfies f1 c)
+    | AND_FORMULA f1 f2     => and(satisfies f1 c) (satisfies f2 c)  
     | IMPLIES_FORMULA f1 f2 => (satisfies f1 c) -> (satisfies f2 c)
    end.
 
-
 (*a well-typed formula only contains names from the feature model*)
 Lemma formNames : forall (fm : FM) (f : Formula),  
- (wt (names_ fm) f) -> ( forall (n : Name),
- set_In n (names f) -> set_In n (names_ fm)).
+ (wt fm f) -> ( forall (n : Name), set_In n (names_ f) -> set_In n (fst fm)).
 Proof.
-  induction f.
-    + simpl; tauto.
-    + simpl; tauto.
-    + simpl. intros. intuition. rewrite H1 in H. apply H.
-    + simpl. tauto.
-    + simpl. intros H ; destruct H. intros. apply set_union_elim in H1. inversion H1.
+induction f.
+   + simpl. intuition.
+   + simpl. intuition.
+   + simpl. intuition. rewrite H1 in H. apply H.
+   + intuition.
+   + simpl. intros H ; destruct H. intros. apply set_union_elim in H1. inversion H1.
       - apply IHf1. apply H. apply H2.
       - apply set_diff_elim1 in H2. apply IHf2. apply H0. apply H2.
     + simpl. intros H. destruct H. intros. apply set_union_elim in H1. inversion H1.
@@ -68,22 +60,22 @@ Proof.
       - apply set_diff_elim1 in H2. apply IHf2. apply H0. apply H2.
 Qed.
 
-Lemma formNames2 : forall (fm : FM) (f : Formula) (n: Name) ,(wt (names_ fm) f) /\ 
-  (~(set_In n (names_ fm))) -> (~(set_In n (names f))).
-Proof. 
-  unfold not.
-  induction f.
-    + simpl; tauto.
-    + simpl; tauto.
-    + simpl. intros. intuition. rewrite H in H1. apply H2. apply H1.
-    + simpl; tauto.
-    + simpl. intros. destruct H; destruct H. apply set_union_elim in H0. inversion H0.
+Lemma formNames2 : forall (fm : FM) (f : Formula) (n: Name) , and (wt fm f) 
+  (not(set_In n (fst fm))) -> (not(set_In n (names_ f))).
+Proof.
+induction f.
+   + intuition.
+   + intuition.
+   + simpl. intuition. rewrite H in H1. apply H2. apply H1.
+   + intuition.
+   + simpl. intros. destruct H; destruct H.  intuition. apply set_union_elim in H2. inversion H2.
       - apply (IHf1 n). intuition. apply H3.
       - apply set_diff_elim1 in H3. apply (IHf2 n). intuition. apply H3. 
-    + simpl. intros. destruct H. destruct H. apply set_union_elim in H0. inversion H0.
+   + simpl. intros. destruct H. destruct H. intuition. apply set_union_elim in H2. inversion H2.
       - apply (IHf1 n). intuition. apply H3.
-      - apply set_diff_elim1 in H3. apply (IHf2 n). intuition. apply H3. 
-Qed.
+      - apply set_diff_elim1 in H3. apply (IHf2 n). intuition. apply H3.
+Qed. 
+
 
 Theorem not_compat : forall A B : Prop,
   (A = B) -> ((~ A) = (~B)).
@@ -96,8 +88,7 @@ Qed.
 
 Lemma set_union_elim_not :
    forall (a:Name) (x y:set Name),
-     ~(set_In a (set_union name_dec x y)) -> 
-        ~(set_In a x) /\ ~(set_In a y).
+     ~(set_In a (set_union name_dec x y)) -> ~(set_In a x) /\ ~(set_In a y).
 Proof.
   intros. split.
     + intuition. apply H. apply set_union_intro1. apply H0.
@@ -106,8 +97,7 @@ Qed.
 
 Lemma set_union_elim_not2 :
    forall (a:Name) (x y:set Name),
-     ~(set_In a x) /\ ~(set_In a y) ->
-      ~(set_In a (set_union name_dec x y)).
+     ~(set_In a x) /\ ~(set_In a y) ->  ~(set_In a (set_union name_dec x y)).
 Proof.  
   intros. destruct H.
   intuition. apply H. 
@@ -119,12 +109,12 @@ Theorem or_commut : forall P Q : Prop,
   P \/ Q -> Q \/ P.
 Proof.
   intros P Q H.
-  tauto. Qed.
+  tauto. Qed. 
+
 
 Lemma set_diff_elim_not:
     forall (n : Name) (f1 f2 : Formula),
-    ~ set_In n (set_diff name_dec (names f1) (names f2)) ->
-    ~ set_In n (names f1) \/ set_In n (names f2).
+    (not (set_In n (set_diff name_dec (names_ f1) (names_ f2)))) -> or (not (set_In n (names_ f1))) (set_In n (names_ f2)).
 Proof.
   intros. left.
   intuition. apply H.
@@ -135,15 +125,14 @@ Proof.
   apply H0.
 Admitted.
 
+(* satisfies's result is equal if we add a feature to the configuration that is not in the formula *)
 Lemma satisfies1 : forall (f: Formula) (c : Configuration) (n : Name),
-  ~(set_In n (names f)) -> satisfies f c = satisfies f (set_add name_dec n c).
+  not(set_In n (names_ f)) -> satisfies f c = satisfies f (set_add name_dec n c).
 Proof.
 induction f. 
-  + simpl; intros; reflexivity.
-  + simpl; intros; reflexivity.
-  + simpl. intros. intuition. apply H1 in H0. 
-    - contradiction. 
-    - rewrite n. rewrite n0. reflexivity.
+  + intuition.
+  + intuition.
+  + simpl. intuition. exfalso. apply H0. rewrite n. rewrite n0. reflexivity.
   + simpl. intros. apply not_compat. apply (IHf c). apply H.
   + simpl. intros. apply set_union_elim_not in H. destruct H as [H1 H2]. 
     specialize (IHf1 c n). specialize (IHf2 c n).
@@ -158,16 +147,16 @@ induction f.
       rewrite H. reflexivity.
     - contradiction.
 Qed.
-    
+
+(*satisfies's result is equal if we remove a feature from the configuration that is not in the formula*)
 Lemma satisfies2 : forall (f: Formula) (c : Configuration) (n : Name),
-  ~(set_In n (names f)) -> satisfies f c = satisfies f (set_remove name_dec n c).
-induction f.
-  + simpl. intros. reflexivity.
-  + simpl. intros. reflexivity.
-  + simpl. intros. intuition. apply H1 in H0. 
-    - contradiction. 
-    - rewrite n. rewrite n0. reflexivity.
-  + simpl. intros. apply not_compat. apply (IHf c). apply H. 
+  not(set_In n (names_ f)) -> satisfies f c = satisfies f (set_remove name_dec n c).
+Proof.
+induction f. 
+  + intuition.
+  + intuition.
+  + simpl. intuition. exfalso. apply H0. rewrite n. rewrite n0. reflexivity.
+  + simpl. intros. apply not_compat. apply (IHf c). apply H.
   + simpl. intros. apply set_union_elim_not in H. destruct H as [H1 H2]. 
     specialize (IHf1 c n). specialize (IHf2 c n).
     apply set_diff_elim_not in H2. inversion H2.
@@ -182,20 +171,23 @@ induction f.
     - contradiction.
 Qed.
 
-Lemma wtFormSameFeature : forall (abs : FM) (con : FM), (names_ abs = names_ con
-  /\ (wfTree abs) /\ (wfTree con) -> forall (f : Formula), (wt (names_ abs) f)
-  ->  (wt (names_ con) f)).
+(* well-typed formulae from a FM continue well-typed in another FM with the same features *)
+Lemma wtFormSameFeature : forall (abs : FM) (con : FM), (fst abs = fst con
+  /\ (wfTree abs) /\ (wfTree con) -> ( forall (f : Formula), (wt abs f) ->  (wt con f))).
 Proof.
   intros.
   destruct H as [equals_abs_con wf_abs_con].
   destruct wf_abs_con as [wf_abs wf_con].
   induction f.
-    + rewrite equals_abs_con in H0. apply H0. 
-    + rewrite equals_abs_con in H0. apply H0. 
+    + auto. 
+    + auto. 
     + simpl. simpl in H0. rewrite equals_abs_con in H0. apply H0. 
-    + apply IHf. apply H0. 
-    + rewrite equals_abs_con in H0. apply H0. 
-    + rewrite equals_abs_con in H0. apply H0. 
+    + auto. 
+    + induction abs, con. simpl. destruct H0. intuition. 
+    + induction abs, con. simpl. destruct H0. intuition. 
 Qed.
 
 End FormulaTheory.
+
+
+
