spl_refinement.v
@@ -1,7 +1,5 @@
 Module SPLrefinement. 
 Require Export maps.
-
-
   Import Maps.
   Require Import Coq.Lists.ListSet.
 
@@ -12,6 +10,7 @@ Require Export maps.
  Inductive Conf: Type.
  Inductive FM: Type.
  
+(*semantic*)
 Parameter inline FMRef : 
     FM -> set Conf.
 
@@ -51,7 +50,8 @@ Axiom conf_dec : forall x y:Conf, {x = y} + {x <> y}.
       + reflexivity.
     Qed.
 
-(*   % Theorems <Feature model equivalence and refinement properties> *)
+(* Theorems <Feature model equivalence and refinement properties> *)
+(* From equivalentFMs -> reflexivity, symmetry, and transitivity *)
   Theorem eqFM:
     forall fm1, equivalentFMs fm1 fm1 /\
       (forall fm1 fm2,equivalentFMs fm1 fm2 -> equivalentFMs fm2 fm1) /\
@@ -73,6 +73,10 @@ Axiom conf_dec : forall x y:Conf, {x = y} + {x <> y}.
     intros. rewrite fm3, fm0. rewrite fm3 in H. rewrite fm4 in H. apply H.
     Qed.
 
+(* mostrar que refinamento de FMs eh partial order nao rola, 
+pois no caso a gente so tem que a semantica seria igual,
+ nao implica que x e y sao iguais*)
+
 (* ===================== Asset MApping ==========================*)
 
   Definition Asset : Type := Maps.T.
@@ -89,8 +93,18 @@ Axiom conf_dec : forall x y:Conf, {x = y} + {x <> y}.
   Parameter assetRef : 
     set Asset -> set Asset -> Prop.
 
+(*a wf function specifying wellformedness of asset sets;
+  this can correspond to the well known notion of type 
+  checking in most languages, but as we do not specify its
+  implementation, it can go beyond that and
+  consider both syntactic and semantic validity*)
   Inductive wfProduct (aSet : set Asset) : Prop.
   Definition Product (aSet : set Asset) : Type := wfProduct aSet.
+
+  Lemma wfaux: forall aSet, True -> wfProduct aSet.
+  Proof.
+  intuition.
+  Qed.
 
 
   Axiom assetRefinementReflexivity:
@@ -103,6 +117,8 @@ Axiom conf_dec : forall x y:Conf, {x = y} + {x <> y}.
   Axiom an_dec : forall x y:AssetName, {x = y} + {x <> y}.
 
 
+(*Such a compositionality property is essential to guarantee independent 
+  development of assets in a product line*)
   Axiom asRefCompositional :
     forall (S1 : set Asset) (S2 : set Asset) (aSet : set Asset),
       (assetRef S1 S2) /\ wfProduct (set_union as_dec S1 aSet) 
@@ -159,14 +175,12 @@ Axiom conf_dec : forall x y:Conf, {x = y} + {x <> y}.
 (* ========================= CK ============================*)
 
  Inductive CK: Type.
- Parameter CKSem : 
-  CK -> AM -> Conf -> set Asset.
+ Parameter CKSem :  CK -> AM -> Conf -> set Asset.
 
   (* Axiom over ck evaluation *)
   Axiom amRef: forall (am1 am2: AM),
-    (aMR am1 am2) -> forall (K: CK) (C: Conf),
-      wfProduct (CKSem K am1 C) -> wfProduct (CKSem K am2 C)
-      /\ assetRef (CKSem K am1 C) (CKSem K am2 C).
+    (aMR am1 am2) -> forall (K: CK) (C: Conf),  wfProduct (CKSem K am1 C) 
+      -> wfProduct (CKSem K am2 C) /\ assetRef (CKSem K am1 C) (CKSem K am2 C).
   
   Variable ck ck1 ck2 ck3: CK.
 
@@ -198,6 +212,20 @@ Axiom conf_dec : forall x y:Conf, {x = y} + {x <> y}.
       - reflexivity.
      Qed. 
 
+
+ Lemma equalsCK2:
+  forall ck1 ck2, equivalentCKs ck1 ck2 -> ck1 = ck2.
+    Proof.
+    unfold equivalentCKs. 
+    unfold equivalentCKsAux. intros. destruct H.
+    (*+ rewrite equalsSetDiff.
+      - trivial.
+      - reflexivity.
+    + rewrite equalsSetDiff.
+      - trivial.
+      - reflexivity. *)
+     Admitted. 
+
   Theorem eqCK:
     forall ck1, equivalentCKs ck1 ck1 /\
       (forall ck1 ck2, equivalentCKs ck1 ck2 -> equivalentCKs ck2 ck1) /\
@@ -214,14 +242,12 @@ Axiom conf_dec : forall x y:Conf, {x = y} + {x <> y}.
 
   Definition weakerEqCK (fm: FM) (ck1 ck2: CK): Prop :=
     forall am,
-      forall c, set_In c (FMRef fm) ->
-        (CKSem ck1 am c = CKSem ck2 am c).
+      forall c, set_In c (FMRef fm) -> (CKSem ck1 am c = CKSem ck2 am c).
 
   
   (* Weak Equivalence properties - reflexive *)
   Theorem weakerEqReflexive:
-    forall (fm: FM) (ck: CK),
-      weakerEqCK fm ck ck.
+    forall (fm: FM) (ck: CK), weakerEqCK fm ck ck.
   Proof.
   intros. unfold weakerEqCK. intros. reflexivity.
   Qed.
@@ -257,20 +283,12 @@ Axiom conf_dec : forall x y:Conf, {x = y} + {x <> y}.
 
 
   Definition wfPL (pl:ArbitrarySPL): Prop :=
-    (forall c, set_In c (FMRef (getFM pl)) ->
-      wfProduct (CKSem (getCK pl) (getAM pl) c)).
+    (forall c, set_In c (FMRef (getFM pl)) -> wfProduct (CKSem (getCK pl) (getAM pl) c)).
 
   (* Definition <Product line> *) 
   Record PL: Type := {
         pls:> ArbitrarySPL;
         wfpl:> Prop }.
-
-  Variable a : ArbitrarySPL.
-
-
-  Definition ase (pl: PL): PL := {| pls:= a; wfpl:= wfPL a |}. 
-
-  (*Definition PL : Type := ArbitrarySPL.*)
 
   Variable pl pl1 pl2: PL.
 
@@ -288,9 +306,7 @@ Axiom conf_dec : forall x y:Conf, {x = y} + {x <> y}.
   (* checar se ainda ha simbolo para ser usado aqui *)
   Definition plRefinement (pl1 pl2: PL): Prop :=
       (forall c1, set_In c1 (FMRef (getFM pl1)) ->
-        (exists c2, set_In c2 (FMRef (getFM pl2)) /\
-          ( assetRef (CKSem (getCK pl1) (getAM pl1) (c1)) 
-              (CKSem (getCK pl2) (getAM pl2) (c2))))). 
+        (exists c2, set_In c2 (FMRef (getFM pl2)) /\ ( assetRef (CKSem (getCK pl1) (getAM pl1) (c1))  (CKSem (getCK pl2) (getAM pl2) (c2))))). 
 
   Axiom confs_dec : forall x y:set Conf, {x = y} + {x <> y}.
 
@@ -323,22 +339,18 @@ Axiom conf_dec : forall x y:Conf, {x = y} + {x <> y}.
 
   Definition  plRefinementAlt (pl1 pl2 : PL) : Prop :=  
     (forall p1: set Asset, set_diff as_dec p1 (products pl1) = nil -> 
-      (exists p2: set Asset, set_diff as_dec p2 (products pl2) = nil /\
-        (assetRef p1 p2))).
+      (exists p2: set Asset, set_diff as_dec p2 (products pl2) = nil /\  (assetRef p1 p2))).
 
   Definition subsetProducts (pl :PL) (prods: set Asset): Prop :=
     set_diff as_dec prods (products pl1) = nil.
 
   Definition plWeakRefinement (pl1 pl2: PL) : Prop :=
     forall p1, set_In p1 (genConf (products pl1))->
-      exists p2, set_In p2 (products pl2) /\
-        (assetRef (set_add as_dec p1 nil) (set_add as_dec p2 nil)). 
+      exists p2, set_In p2 (products pl2) /\ (assetRef (set_add as_dec p1 nil) (set_add as_dec p2 nil)). 
 
   Definition strongerPLrefinement (pl1 pl2:PL) : Prop :=
     forall c1: Conf, set_In c1 (FMRef (getFM pl1)) ->
-      (set_In c1 (FMRef (getFM pl2)) /\
-          (assetRef (CKSem (getCK pl1) (getAM pl1) c1)
-               (CKSem (getCK pl2) (getAM pl2) c1))).
+      (set_In c1 (FMRef (getFM pl2)) /\ (assetRef (CKSem (getCK pl1) (getAM pl1) c1) (CKSem (getCK pl2) (getAM pl2) c1))).
   
   Theorem plStrongSubset:
     forall (pl1 pl2: PL),
@@ -384,7 +396,7 @@ Axiom conf_dec : forall x y:Conf, {x = y} + {x <> y}.
       -  unfold getFM. simpl.  unfold getFM in H0. destruct pl0 in H0.
         simpl in H0. destruct pls0 in H0. simpl in H0. destruct p0. rewrite f in H0.
         rewrite fm0. apply H0.
-      - unfold getCK. unfold getAM. simpl.
+      - unfold getCK. unfold getAM. simpl. 
         apply assetRefinementReflexivity.
     + unfold wfPL. intros.
       unfold equivalentFMs in H.
@@ -396,16 +408,21 @@ Axiom conf_dec : forall x y:Conf, {x = y} + {x <> y}.
   Theorem ckEquivalenceCompositionality:
     forall (pl: PL) (ck: CK),
       equivalentCKs (getCK pl) ck ->
-        (plRefinement pl {| pls:= ((fm ,(getAM pl)), (getCK pl)); wfpl := wfPL ((fm ,(getAM pl)), (getCK pl))|})
-         /\ wfPL ((fm ,(getAM pl)), (getCK pl)).
+        (plRefinement pl {| pls:= (((getFM pl) ,(getAM pl)), ck); wfpl := wfPL (((getFM pl) ,(getAM pl)), ck)|})
+         /\ wfPL (((getFM pl) ,(getAM pl)), ck).
     Proof.
     intros.
     split.
     + unfold plRefinement. intros. exists c4. split.
       -  unfold getFM. simpl.  unfold getFM in H0. destruct pl0 in H0.
         simpl in H0. destruct pls0 in H0. simpl in H0. destruct p0. simpl in H0. rewrite f in H0.
-        rewrite fm. apply H0.
-      - unfold getCK. unfold getAM. simpl.
+        destruct pl0. simpl. destruct pls0. simpl. destruct p0. simpl. destruct f0.        
+        apply H0.
+      - unfold getFM. unfold getAM. simpl. unfold getCK. destruct pl0.
+        simpl. destruct pls0. simpl.  destruct c0 in H0. destruct p0. simpl in H0.
+        unfold getFM in H0. simpl in H0. destruct f. simpl. destruct c4. 
+        intuition. Search assetRef. unfold getCK in H.
+        simpl in H. Search equivalentCKs. apply equalsCK2 in H. rewrite H.
         apply assetRefinementReflexivity.
     + unfold wfPL. intros.
       unfold equivalentFMs in H.
@@ -415,16 +432,22 @@ Axiom conf_dec : forall x y:Conf, {x = y} + {x <> y}.
   Theorem weakerCKcompositionality:
     forall (pl: PL) (ck: CK),
       weakerEqCK (getFM pl) (getCK pl) (ck) ->
-        plRefinement pl {|pls := ((fm ,(getAM pl)), (getCK pl)); wfpl := wfPL ((fm ,(getAM pl)), (getCK pl))|}
-         /\ wfPL ((fm ,(getAM pl)), (getCK pl)).
+        (plRefinement pl {| pls:= (((getFM pl) ,(getAM pl)), ck); wfpl := wfPL (((getFM pl) ,(getAM pl)), ck)|})
+         /\ wfPL (((getFM pl) ,(getAM pl)), ck).
     Proof.
     intros.
     split.
     + unfold plRefinement. intros. exists c4. split.
-      -  unfold getFM. simpl.  unfold getFM in H0. destruct pl0 in H0.
-        simpl in H0. destruct pls0 in H0. simpl in H0. destruct p0. rewrite f in H0.
-        rewrite fm. apply H0.
-      - unfold getCK. unfold getAM. simpl.
+      - unfold getFM. simpl.  unfold getFM in H0. destruct pl0 in H0.
+        simpl in H0. destruct pls0 in H0. simpl in H0. destruct p0. simpl in H0. rewrite f in H0.
+        destruct pl0. simpl. destruct pls0. simpl. destruct p0. simpl. destruct f0.        
+        apply H0.
+      - unfold getFM. unfold getAM. simpl. unfold getCK. destruct pl0.
+        simpl. destruct pls0. simpl.  destruct c0 in H0. destruct p0. simpl in H0.
+        unfold getFM in H0. simpl in H0. destruct f. simpl. destruct c4. 
+        intuition. Search assetRef. unfold getFM in H.
+        simpl in H. unfold weakerEqCK in H. specialize (H a c).
+        destruct c. intuition. rewrite H1.
         apply assetRefinementReflexivity.
     + unfold wfPL. intros.
       unfold equivalentFMs in H.
@@ -436,19 +459,20 @@ Axiom conf_dec : forall x y:Conf, {x = y} + {x <> y}.
   Theorem amRefinementCompositionality:
     forall (pl: PL) (am: AM),
       aMR (getAM pl) am ->
-        plRefinement pl {| pls := ((fm ,(getAM pl)), (getCK pl)); wfpl:= wfPL ((fm ,(getAM pl)), (getCK pl))|}
-         /\
-           wfPL ((fm ,(getAM pl)), (getCK pl)).
-    Proof.
+        plRefinement pl {| pls := ((getFM pl), am, (getCK pl)); wfpl:= wfPL ((getFM pl) , am, (getCK pl))|}
+         /\ wfPL ((getFM pl) ,am, (getCK pl)).
+    Proof. 
     intros.
     split.
-    + unfold plRefinement. intros. exists c4. split.
-      -  unfold getFM. simpl.  unfold getFM in H0. destruct pl0 in H0.
-        simpl in H0. destruct pls0 in H0. simpl in H0. destruct p0 in H0. simpl in H0.
-        rewrite f in H0.
-        rewrite fm. apply H0.
-      - unfold getCK. unfold getAM. simpl.
-        apply assetRefinementReflexivity.
+    +   unfold plRefinement. Search aMR.  intros. exists c4. split.
+      - unfold getFM. simpl.  unfold getFM in H0. destruct pl0 in H0.
+        simpl in H0. destruct pls0 in H0. simpl in H0. destruct p0. simpl in H0. rewrite f in H0.
+        destruct pl0. simpl. destruct pls0. simpl. destruct p0. simpl. destruct f0.        
+        apply H0.
+      -  unfold getCK. unfold getAM. simpl. Search aMR. apply amRef.
+          * apply H.
+          *  destruct pl0. simpl. destruct pls0. simpl. destruct p0.
+            simpl. simpl in H, H0. apply wfaux. intuition.
     + unfold wfPL. intros.
       unfold equivalentFMs in H.
       destruct H. intuition.
@@ -462,9 +486,8 @@ Axiom conf_dec : forall x y:Conf, {x = y} + {x <> y}.
       equivalentFMs (getFM pl) fm /\
         equivalentCKs (getCK pl) ck /\
           aMR (getAM pl) am ->
-            plRefinement pl {| pls := ((fm ,(getAM pl)), (getCK pl)); 
-              wfpl:= wfPL ((fm ,(getAM pl)), (getCK pl))|}  /\
-                wfPL ((fm ,(getAM pl)), (getCK pl)).
+            plRefinement pl {| pls := (fm ,am, ck); wfpl:= wfPL (fm ,am, ck)|}  /\
+                wfPL (fm ,am, ck).
     Proof.
     intros.
     split.
@@ -473,8 +496,14 @@ Axiom conf_dec : forall x y:Conf, {x = y} + {x <> y}.
         simpl in H0. destruct pls0 in H0. simpl in H0. destruct p0. simpl in H0.
         rewrite f in H0.
         rewrite fm0. apply H0.
-      - unfold getCK. unfold getAM. simpl.
-        apply assetRefinementReflexivity.
+      - unfold getCK. unfold getAM. simpl. destruct H.
+        intuition. Search assetRef. unfold getCK in H2.
+        simpl in H2. apply equalsCK2 in H2. rewrite H2. 
+        destruct pl0. simpl in H, H0, H2, H3. simpl. unfold getAM in H3.
+        simpl. 
+        destruct pls0. simpl. apply amRef.
+        * simpl in H3. apply H3.
+        *  destruct p0. simpl. simpl in H, H0, H2, H3. apply wfaux. intuition.
     + unfold wfPL. intros.
       unfold equivalentFMs in H.
       destruct H. intuition.
@@ -488,9 +517,10 @@ Axiom conf_dec : forall x y:Conf, {x = y} + {x <> y}.
     forall (pl: PL) (fm: FM) (am: AM) (ck: CK),
       (FMRefinement (getFM pl) fm) /\
         equivalentCKs (getCK pl) ck /\
-           wfPL ((fm ,(getAM pl)), (getCK pl)) ->
-             plRefinement pl {| pls := ((fm ,(getAM pl)), (getCK pl));
-               wfpl := wfPL ((fm ,(getAM pl)), (getCK pl)) |}.
+          aMR (getAM pl) am /\
+           wfPL (fm ,am, ck) ->
+             plRefinement pl {| pls := (fm ,am, ck);
+               wfpl := wfPL (fm ,am, ck) |}.
     Proof.
     intros. 
     destruct H.   
@@ -500,9 +530,13 @@ Axiom conf_dec : forall x y:Conf, {x = y} + {x <> y}.
         simpl in H1. destruct pls0 in H1. simpl in H1. destruct p0. simpl in H1.
         rewrite f in H1.
         rewrite fm0. apply H1. 
-      + unfold getCK. unfold getAM. simpl.
-        apply assetRefinementReflexivity.
-    Qed.
+      + unfold getCK. unfold getAM. unfold wfPL in H0.
+        destruct H0. unfold getCK in H0.
+        simpl in H0. apply equalsCK2 in H0. rewrite H0. 
+        destruct pl0. simpl in H, H0, H2. simpl. apply amRef.
+        * destruct H2. unfold getAM in H2. apply H2.
+        *   simpl. simpl in H, H0, H2. apply wfaux. intuition.
+  Qed.
 
   (*Theorem <Full compositionality>
   Este teorema exige a equivalencia mais fraca de CK e equivalencia de FMs *)
@@ -512,9 +546,9 @@ Axiom conf_dec : forall x y:Conf, {x = y} + {x <> y}.
       equivalentFMs (getFM pl) fm /\
         weakerEqCK (getFM pl) (getCK pl) (ck) /\ 
           aMR (getAM pl) am ->
-            plRefinement pl  {| pls := ((fm ,(getAM pl)), (getCK pl));
-              wfpl:= wfPL ((fm ,(getAM pl)), (getCK pl))|} /\
-              wfPL ((fm ,(getAM pl)), (getCK pl)).
+            plRefinement pl  {| pls := (fm ,am, ck);
+              wfpl:= wfPL (fm ,am, ck)|} /\
+              wfPL (fm , am, ck).
     Proof.
     intros.
     split.
@@ -523,8 +557,14 @@ Axiom conf_dec : forall x y:Conf, {x = y} + {x <> y}.
         simpl in H0. destruct pls0 in H0. simpl in H0. destruct p0. 
         simpl in H0. rewrite f in H0.
         rewrite fm0. apply H0.
-      - unfold getCK. unfold getAM. simpl.
-        apply assetRefinementReflexivity.
+      - unfold getCK. unfold getAM. simpl. destruct H.
+        destruct H1.  unfold weakerEqCK in H1. destruct pl0. destruct pls0.
+        destruct p0. simpl.
+        simpl in H, H1, H2, H0. specialize (H1 a c4). intuition.
+        rewrite H3. apply amRef. 
+        * unfold getAM in H2. simpl in H2.
+        apply H2.
+        * simpl. simpl in H, H0, H2. apply wfaux. intuition.
     + unfold wfPL. intros.
       unfold equivalentFMs in H.
       destruct H. intuition.
@@ -536,9 +576,10 @@ Axiom conf_dec : forall x y:Conf, {x = y} + {x <> y}.
      Theorem weakFullCompositionality2:
         forall (pl: PL) (fm: FM) (am: AM) (ck: CK),       
           (FMRefinement (getFM pl) fm) /\
-            aMR (getAM pl) am /\ wfPL ((fm ,(getAM pl)), (getCK pl)) ->
-              plRefinement pl {| pls := ((fm ,(getAM pl)), (getCK pl)); 
-                wfpl := wfPL ((fm ,(getAM pl)), (getCK pl))|}.
+            weakerEqCK (getFM pl) (getCK pl) (ck) /\ 
+             aMR (getAM pl) am /\ wfPL ((fm ,(getAM pl)), (getCK pl)) ->
+              plRefinement pl {| pls := (fm ,am, ck); 
+                wfpl := wfPL (fm , am, ck)|}.
     Proof.
     intros. 
     destruct H.   
@@ -548,9 +589,15 @@ Axiom conf_dec : forall x y:Conf, {x = y} + {x <> y}.
         simpl in H1.  destruct pls0 in H1. simpl in H1. destruct p0. simpl in H1.
         rewrite f in H1.
         rewrite fm0. apply H1.  
-      + unfold getCK. unfold getAM. simpl.
-        apply assetRefinementReflexivity.
-    Qed.
+      + unfold getCK. unfold getAM. simpl. destruct H0.
+        destruct H2.  unfold weakerEqCK in H0. destruct pl0. destruct pls0.
+        destruct p0. simpl.
+        simpl in H, H1, H2, H0, H3. specialize (H0 a c4). intuition.
+        rewrite H4. apply amRef. 
+        * unfold getAM in H2. simpl in H2.
+        apply H2.
+        * simpl. apply wfaux. intuition.
+  Qed.
 
      Lemma equalsRefinementAlt:
       forall pl1 pl2, pl1 = pl2-> plRefinementAlt pl1 pl2.
@@ -619,8 +666,7 @@ Axiom conf_dec : forall x y:Conf, {x = y} + {x <> y}.
 
    Theorem plRef:
       forall pl1, plRefinement pl1 pl1 /\
-        (forall pl1 pl2 pl3: PL, plRefinement pl1 pl2 /\
-          plRefinement pl2 pl3 -> plRefinement pl1 pl3).
+        (forall pl1 pl2 pl3: PL, plRefinement pl1 pl2 /\ plRefinement pl2 pl3 -> plRefinement pl1 pl3).
       Proof.
       intros.
       split.
