Specific_SPL.v
@@ -1,0 +1,615 @@
+Module SpecificSPL. 
+
+Require Export maps_int formulatheory_int featuremodelsemantics_int assettheory_int
+               assetmapping_int featuremodelrefinement_int.
+
+Require Export maps_def formulatheory_def featuremodelsemantics_def featuremodelrefinement_def
+               assettheory_def assetmapping_def ckcomp_int ckcomp_def.
+
+Import FormulaTheory FeatureModelSemantics AssetTheory AssetMapping CKComp
+       Maps FeatureModelRefinimentTheory.
+
+Require Export formulatheory_inst featuremodelsemantics_inst assettheory_inst maps_inst
+               assetmapping_inst featuremodelrefinement_inst  ckcomp_inst.
+
+Require Import Coq.Lists.ListSet.
+
+  Variable fm fm1 fm2: FM.
+  Variable am am1 am2 pairs: AM.
+  Variable ck ck1 ck2: CK.
+  Variable item item1 item2: Item.
+  Variable items items1 items2: set Item. 
+  Variable c c1 c2: Configuration.
+  Variable expr: Formula.
+  Variable Fe G H opt: Name.
+  Variable a a1 a2 a3: Asset.
+  Variable an an1 an2: AssetName.
+
+
+  Axiom item_dec : forall x y:Item, {x = y} + {x <> y}.
+  Axiom pair_dec : forall x y:pair_, {x = y} + {x <> y}.
+  Axiom ns_dec : forall   x y:Name, {x = y} + {x <> y}.
+  Axiom an_dec : forall   x y:AssetName, {x = y} + {x <> y}.
+  Axiom as_dec : forall   x y:AssetName, {x = y} + {x <> y}.
+
+Require Export spl_int spl_def spl_proofs spl_inst.
+Import SPL.
+
+  (*========= IF WE ADD NEW ASSETS TO AM THAT DID NOT EXIST BEFORE, 
+              CK EVALUATION IS THE SAME =============*)
+  Lemma mapSubsetAM :
+   forall fm am1 am2 ck,
+    forall an, set_In an (dom_func am2) -> ~(set_In an (dom_func am1)) /\
+      wfCK_func fm am1 ck   
+        -> forall (c: Configuration), set_In c (semantics fm)
+          -> (semantics_func_ ck am1 c =
+              semantics_func_ ck (set_union pair_dec am1 am2) c).
+  Proof.
+  unfold wfCK_func.
+  induction am4.
+  + induction am3.
+    - simpl. intuition.
+    - simpl. intuition. 
+  + intuition. specialize (IHam4 ck0 an0). 
+    apply set_add_elim in H0. intuition.
+Admitted. 
+
+ (*============= REPLACE FEATURE EXPRESSION ==================*)
+
+
+  Definition syntaxReplaceFeatureExp ck1 ck2 item1 item2 items: Prop:=
+    (ck1 =  app (items :: nil) (item1 :: nil) ) /\
+      (ck2 = app (items :: nil) (item2 :: nil)) /\
+        item1.(assets) = item2.(assets).  
+ 
+ Definition conditionsReplaceFeatureExp (fm:FM) item1 item2: Prop :=
+    wt fm (item2.(exp)) /\
+      forall c, set_In c (semantics fm) ->
+        iff (satisfies (item1.(exp)) c) (satisfies (item2.(exp)) c).  
+
+ Theorem replaceFeatureExp_EqualCKeval 
+    {Mp: Maps Asset AssetName AM}
+      {Ft: FormulaTheory Formula Name FM}
+        {FtM: FeatureModel FM Configuration} 
+          {AssetM: AssetMapping Asset AssetName AM} 
+            {ckTrans: CKTrans FM Asset AM CK Configuration} 
+              {SPL: SPL Asset Configuration FM AM CK PL}: 
+    forall (pl: PL) ck2 item1 item2 items,
+      (
+        (
+         wfCK_func (getFM pl) (getAM pl) (getCK pl) /\
+          syntaxReplaceFeatureExp (getCK pl) ck2 item1 item2 items /\
+           conditionsReplaceFeatureExp (getFM pl) item1 item2
+       )
+         ->
+          forall (c: Configuration), set_In c (semantics (getFM pl))
+            -> semantics_ (getCK pl)(getAM pl) c 
+              = semantics_ ck2 (getAM pl) c
+       ).
+  Proof.
+  intros. destruct H0. destruct H2. 
+  unfold syntaxReplaceFeatureExp in H2. destruct H2.
+  destruct H4. rewrite H4. rewrite H2. simpl. 
+  induction item4. induction item3.
+  simpl in H5. rewrite H5.  intuition. 
+  Qed.
+
+ Theorem replaceFeatureExpression 
+    {Mp: Maps Asset AssetName AM}
+      {Ft: FormulaTheory Formula Name FM}
+        {FtM: FeatureModel FM Configuration} 
+          {AssetM: AssetMapping Asset AssetName AM} 
+            {ckTrans: CKTrans FM Asset AM CK Configuration} 
+              {SPL: SPL Asset Configuration FM AM CK PL}: 
+    forall (pl: PL) ck2 item1 item2 items,
+      (
+        (
+         wfCK_func (getFM pl) (getAM pl) (getCK pl) /\
+          syntaxReplaceFeatureExp (getCK pl) ck2 item1 item2 items /\
+           conditionsReplaceFeatureExp (getFM pl) item1 item2
+       )
+         ->
+          plRefinement_func pl (gerPL fm2 (getAM pl) ck2) /\
+          wfCK_func (getFM pl) (getAM pl) ck2 /\
+          wfPL (gerPL fm2 (getAM pl) ck2)         
+       ).
+  Proof.
+  intuition.
+  + unfold plRefinement_func.  intros. exists c3. split.
+      -  destruct gerPL. unfold getFM_func. simpl.  unfold getFM_func in H2. destruct pl in H2. 
+        simpl in H2. destruct pls1. simpl in H2. destruct p.
+        destruct pls0.  simpl in H2. destruct p.
+        simpl in H2. destruct f, f0. simpl. apply H2. 
+  (*    -  
+
+specialize (H7 an). destruct H7. destruct H10. destruct G, F.
+        intuition.
+  + intros. unfold syntaxReplaceFeatureExp in H0. destruct H0.
+  destruct H2. rewrite H2.
+  symmetry in H4. simpl.
+  induction item4. induction item3.
+  simpl in H4, H1, H2, H3. rewrite H4. intuition.
+  Search wfCK_func. rewrite H0 in H1.
+  simpl in H1. unfold conditionsReplaceFeatureExp in H3.
+  destruct H3. Search satisfies.*)
+Admitted.
+
+
+ (*==================  ADD MANDATORY FEATURE ======================*)
+
+
+(* FOR ALL PRODUCTS OF A FM, EVALUATING THE CK WITH A DEAD FEATURE IS EQUIVALENT TO EVALUATING THE CK WITHOUT IT*)
+
+ Theorem evalCKdeadFeature 
+  {Mp: Maps Asset AssetName AM}
+    {Ft: FormulaTheory Formula Name FM}
+      {FtM: FeatureModel FM Configuration} 
+        {AssetM: AssetMapping Asset AssetName AM} 
+          {ckTrans: CKTrans FM Asset AM CK Configuration} 
+            {SPL: SPL Asset Configuration FM AM CK PL} 
+              {FormT: FormulaTheory Formula Name FM}
+                {FMS: FeatureModelSemantics Formula FM Name}
+                  {FMR: FeatureModelRefinement Formula Name FM}:
+    forall pl (opt: Name),
+      ~(set_In opt (nsf_func ((fst(fst pl))))) /\
+        wfCK (fst(fst pl)) (snd(fst pl)) (snd pl) 
+          -> forall c, set_In c (semantics_func (fst(fst pl)))
+            -> semantics_func_ (snd pl) (snd(fst pl)) c = 
+              semantics_func_ (snd pl) (snd(fst pl)) (app (opt:: nil) c). 
+  Proof. 
+  simpl. intuition. simpl. simpl in H1, H2, H0. unfold nsf_func in H1. 
+  destruct a4. simpl in H1, H2, H0. destruct f. intuition.
+  destruct opt0, n.  simpl in H1. intuition.  
+  Qed.
+
+
+ Definition syntaxConditionsAddMandatoryFeature (fm1 fm2: FM) (F G: Name) 
+  {FormT: FormulaTheory Formula Name FM} {FMS: FeatureModelSemantics Formula FM Name }
+  {FMR: FeatureModelRefinement Formula Name FM}: Prop :=
+    addMandatoryNode_func fm1 fm2 F G. 
+
+
+ (*ADDING A MANDATORY FEATURE G WITHOUT CHANGING CK AND AM IS PL REFINEMENT*)
+
+ Theorem addMandatoryFeat 
+    {Mp: Maps  AssetName Asset AM}
+      {FtM: FeatureModel FM Configuration} 
+        {AssetM: AssetMapping Asset AssetName AM} 
+          {ckTrans: CKTrans FM Asset AM CK Configuration} 
+            {SPL: SPL Asset Configuration FM AM CK PL} 
+              {FormT: FormulaTheory Formula Name FM} 
+                {FMS: FeatureModelSemantics Formula FM Name }
+                  {FMR: FeatureModelRefinement Formula Name FM}:
+    forall (pl: PL) (F G: Name) (fm2: FM),
+      (
+        syntaxConditionsAddMandatoryFeature (getFM pl) fm2 F G /\
+          wfCK (getFM pl) (getAM pl) (getCK pl)
+            ->
+            plRefinement_func pl (gerPL fm2 (getAM pl) (getCK pl)) 
+              /\ wfCK fm2 (getAM pl) (getCK pl)
+                /\ wfPL (gerPL fm2 (getAM pl) (getCK pl))
+       ). 
+  Proof.
+ intuition. simpl. unfold syntaxConditionsAddMandatoryFeature in H1.
+ unfold addMandatoryNode_func in H1. destruct F, G0.
+ intuition. unfold syntaxConditionsAddMandatoryFeature in H1.
+ unfold addMandatoryNode_func in H1. destruct F, G0.
+ intuition. unfold syntaxConditionsAddMandatoryFeature in H1.
+ unfold addMandatoryNode_func in H1. destruct F, G0.
+ intuition.
+Qed.
+
+(* =============SPLIT ASSETS====================*)
+
+  (* SPLIT ASSETS conditions *)
+  
+ Definition syntaxSplitAssets am1 am2 (ck1 ck2:CK) (item1 item2: Item) items
+              (an1 an2: AssetName) (a1 a2 a3: Asset) pairs: Prop :=  
+    am1 = set_add pair_dec (an1, a1)  pairs /\
+    am2 = set_add pair_dec (an1, a2) (set_add pair_dec (an2, a3) pairs) /\
+    ck1 =  app (item1::nil) items /\
+    ck2 = app (item2::nil) items /\
+      item1.(exp) = item2.(exp) /\
+    item1.(assets) =  set_add an_dec an1 nil /\ 
+    item2.(assets) = set_add an_dec an1 (an2::nil). 
+  
+  Definition conditionsSplitAssets a1 a2 a3 an1 an2 items: Prop :=
+    assetRef_func (a1::nil) (app (a2::nil) (a3::nil)) /\
+      forall (item: Item), set_In item items
+        -> ~(set_In an1 (item.(assets))) /\
+          (~ set_In an2 (item.(assets))).  
+
+  Lemma same_add: forall (p:pair_) pairs, set_add pair_dec p pairs = 
+        set_add pair_dec p (set_add pair_dec p pairs).
+  Proof.
+  intros. induction p.
+  unfold set_add. induction pairs0.
+  - case_eq (pair_dec (a0,b) (a0,b)).
+    + intros. reflexivity.
+    + intros. intuition.
+  - intuition. case_eq (pair_dec (a0, b) a4).
+    + intros. rewrite e. case_eq (pair_dec (a0,b) a4).
+      * intros. case_eq (pair_dec a4 a4).
+        { intuition. }
+        { intuition. }
+      * intuition.
+    + intuition. rewrite IHpairs0. intuition.
+      induction a4. simpl. intuition. 
+      case_eq (pair_dec (a0, b) (a4, b0)).
+        {intuition. }
+        { intuition. destruct a0, b, a4, b0. 
+          intuition. }
+Qed.
+
+
+Theorem splitNotEvalItem 
+  {Mp: Maps Asset AssetName AM}
+   {Ft: FormulaTheory Formula Name FM}
+    {FtM: FeatureModel FM Configuration}
+     {AssetM: AssetMapping Asset AssetName AM} 
+      {ckTrans: CKTrans FM Asset AM CK Configuration} 
+       {SPL: SPL Asset Configuration FM AM CK PL}:
+     forall pl am2 ck2 item1 item2 a1 a2 a3 an1 an2 items pairs,
+  (
+    ( 
+        wfCK_func (fst(fst pl)) (snd(fst pl)) (snd pl) /\
+          syntaxSplitAssets (snd(fst pl)) am2 (snd pl) ck2 item1 item2 items an1 an2 a1 a2 a3 pairs /\
+            conditionsSplitAssets a1 a2 a3 an1 an2 items
+    )
+    ->
+      forall c, set_In c (semantics_func (fst(fst pl))) /\
+        ~(satisfies_func (item1.(exp)) c)
+          -> semantics_func_ (snd pl) (snd(fst pl)) c = semantics_func_ ck2 am2 c). 
+  Proof. 
+  destruct pl. destruct p. simpl. destruct f. intros am ck item1 item2 a1 a2 a3 an1 an2 items pairs.
+  unfold syntaxSplitAssets. unfold conditionsSplitAssets. simpl. 
+  intuition. specialize (H5 item1). rewrite H8 in H5.
+  induction item1, item2.
+  simpl in H1, H2, H0, H5, H3, H4, H6, H7, H8, H10, H11, H12. simpl. 
+  intuition. rewrite H4, H2, H6, H3.
+  rewrite H7, H8, H10. rewrite H7, H8 in H5.
+  intuition. case_eq (an_dec an1 an2). 
+  + intros.  rewrite same_add. destruct an1, a1, a2, an2, a3. reflexivity. 
+  + intros. destruct n. destruct an1, an2. reflexivity.
+Qed.
+
+   (*When splitting assets, if item1 is evaluated as true, ck evaluation is equal to the asset mapped by this item union evaluation of other items*)
+
+ Theorem splitEvalItemUnion 
+  {Mp: Maps Asset AssetName AM}
+   {Ft: FormulaTheory Formula Name FM}
+    {FtM: FeatureModel FM Configuration} 
+     {AssetM: AssetMapping Asset AssetName AM} 
+      {ckTrans: CKTrans FM Asset AM CK Configuration} 
+       {SPL: SPL Asset Configuration FM AM CK PL}:
+    forall pl am2 ck2 item1 item2 a1 a2 a3 an1 an2 items pairs,
+    (
+      ( 
+          wfCK (fst(fst pl)) (snd(fst pl)) (snd pl) /\
+          syntaxSplitAssets (snd(fst pl)) am2 (snd pl) ck2 item1 item2 items an1 an2 a1 a2 a3 pairs /\
+            conditionsSplitAssets a1 a2 a3 an1 an2 items
+    )
+    ->
+        forall c, set_In c (semantics_func (fst(fst pl))) /\ ~(satisfies_func (item1.(exp)) c)
+    -> semantics_func_ (snd pl) (snd (fst pl)) c = app (a1::nil) (semantics_func_ items (snd (fst pl)) c) /\
+       semantics_func_ ck2 am2 c = app (app (a2:: nil) (a3::nil)) (semantics_func_ items am2 c)). 
+    Proof. 
+    destruct pl. destruct p. simpl. 
+    intros am ck item1 item2 a1 a2 a3 an1 an2 items pairs.
+    induction item1, item2.
+    unfold syntaxSplitAssets. unfold conditionsSplitAssets. 
+    simpl. intuition.
+  +  rewrite H4. rewrite H8. unfold wfCK_func in H1.
+     destruct H1. destruct H9. specialize (H9 c0).
+     intuition. specialize (H13 exp0). 
+     rewrite H4 in H13. unfold wfFM_func in H1. 
+     destruct H1.
+     unfold wfFormulae_func in H9. specialize (H9 exp0).
+     rewrite H2. simpl.   admit.
+  + rewrite H6. rewrite H10. case_eq (an_dec an1 an2).
+    - intros. admit.
+    - intros. destruct an1, an2. intuition. 
+    Admitted.
+
+ Theorem splitEvalRemainingItems 
+  {Mp: Maps Asset AssetName AM}
+   {Ft: FormulaTheory Formula Name FM}
+    {FtM: FeatureModel FM Configuration} 
+     {AssetM: AssetMapping Asset AssetName AM} 
+      {ckTrans: CKTrans FM Asset AM CK Configuration} 
+       {SPL: SPL Asset Configuration FM AM CK PL}:
+  forall pl am2 ck2 (item1 item2: Item) (a1 a2 a3: Asset) (an1 an2: AssetName) (items: list Item) (pairs: AM),
+    (
+      ( 
+        wfCK (fst(fst pl)) (snd(fst pl)) (snd pl)  /\
+          syntaxSplitAssets (snd(fst pl)) am2 (snd pl) ck2 item1 item2 items an1 an2 a1 a2 a3 pairs /\
+            conditionsSplitAssets a1 a2 a3 an1 an2 items
+    )
+    ->
+      forall c, set_In c (semantics (fst(fst pl))) 
+    ->
+        (semantics_ items (snd(fst pl)) c) = (semantics_ items am2 c)).
+  Proof.
+ destruct pl. destruct p. simpl. destruct f. intros am ck item1 item2 a1 a2 a3 an1 an2 items pairs.
+  unfold syntaxSplitAssets. unfold conditionsSplitAssets. simpl. 
+  intuition. 
+  specialize (H5 item1). rewrite H8 in H5.
+  induction item1, item2.
+  simpl in H1, H2, H0, H5, H3, H4, H6, H7, H8, H10. simpl. 
+  intuition.
+  rewrite H2, H3.
+  rewrite same_add. destruct an1, a1, a2, an2, a3. reflexivity. 
+  Qed.
+
+  
+ (* Split assets preserves CK well-formedness *)
+
+  Theorem splitAssetWFCK 
+    {Mp: Maps Asset AssetName AM}
+      {Ft: FormulaTheory Formula Name FM}
+        {FtM: FeatureModel FM Configuration} 
+          {AssetM: AssetMapping Asset AssetName AM} 
+            {ckTrans: CKTrans FM Asset AM CK Configuration} 
+              {SPL: SPL Asset Configuration FM AM CK PL}:
+    forall pl (am2:AM) (ck2: CK) (item1 item2: Item) (a1 a2 a3: Asset) (an1 an2: AssetName) items pairs,
+    (
+      ( 
+       wfCK_func (fst(fst pl)) (snd(fst pl)) (snd pl)  /\
+          syntaxSplitAssets (snd(fst pl)) am2 (snd pl) ck2 item1 item2 items an1 an2 a1 a2 a3 pairs /\
+            conditionsSplitAssets a1 a2 a3 an1 an2 items
+    )
+    ->
+      wfCK_func (fst(fst pl)) am2 ck2).
+  Proof.
+  destruct pl. destruct p. simpl. destruct f. intros am ck item1 item2 a1 a2 a3 an1 an2 items pairs.
+  unfold syntaxSplitAssets. unfold conditionsSplitAssets. simpl. 
+  intuition. 
+  specialize (H5 item1). rewrite H8 in H5.
+  induction item1, item2.
+  simpl in H1, H2, H0, H5, H3, H4, H6, H7, H8, H10. simpl. 
+  intuition.
+  rewrite H6, H3. rewrite H2, H4 in H1.
+  rewrite H10. rewrite H8 in H1. 
+  intuition. case_eq (an_dec an1 an2). 
+  + intros.  rewrite same_add in H1. destruct an1, a1, a2, an2, a3. rewrite H7 in H1. apply H1. 
+  + intros. destruct n. destruct an1, an2. reflexivity.
+  Qed.
+
+
+ Theorem splitAsset
+    {Mp: Maps Asset AssetName AM}
+      {Ft: FormulaTheory Formula Name FM}
+        {FtM: FeatureModel FM Configuration} 
+          {AssetM: AssetMapping Asset AssetName AM} 
+            {ckTrans: CKTrans FM Asset AM CK Configuration} 
+              {SPL: SPL Asset Configuration FM AM CK PL}:
+    forall (pl:PL) (am2:AM) (ck2: CK) (item1 item2: Item) (a1 a2 a3: Asset) (an1 an2: AssetName) items pairs,
+    (
+      ( 
+       wfCK_func (getFM pl) (getAM pl) (getCK pl)  /\
+          syntaxSplitAssets (getAM pl) am2 (getCK pl) 
+          ck2 item1 item2 items an1 an2 a1 a2 a3 pairs /\
+            conditionsSplitAssets a1 a2 a3 an1 an2 items
+    )
+    ->
+      plRefinement_func pl (gerPL (getFM pl) am2 ck2) /\
+      wfCK_func (getFM pl) am2 ck2) /\
+      wfPL (gerPL (getFM pl) am2 ck2).
+  Proof.
+  intuition.
+  + unfold plRefinement_func. intros. admit.
+  + Search wfCK_func.  
+
+  Admitted.
+
+ (* ================= ADD OPTIONAL FEATURE ==================*)
+
+ Definition syntaxAddOptionalFeature 
+  {FormT: FormulaTheory Formula Name FM}
+   {FMS: FeatureModelSemantics Formula FM Name }
+    {FMR: FeatureModelRefinement Formula Name FM} 
+    (fm1: FM) (am1: AM) (ck1: CK) (fm2: FM) (am2: AM) (ck2: CK) (F G: Name) items (pairs: AM) :Prop :=
+    fst fm2 = app (G::nil)  (fst fm1) /\
+    set_In F (fst fm1) /\
+    (snd fm2) = set_add form_dec (IMPLIES_FORMULA (NAME_FORMULA(G)) (NAME_FORMULA(F))) (snd fm1) /\
+    am2 = app am1 (pairs) /\
+    ck2 = app ck1 items. 
+
+ Definition conditionsAddOptionalFeature (fm1 fm2: FM) (am1 am2 pairs: AM) (ck2: CK) (G: Name) (items: set Item) 
+    {Mp: Maps AssetName Asset AM}
+     {Ft: FormulaTheory Formula Name FM}
+      {FtM: FeatureModel FM Configuration} {AssetM: AssetMapping Asset AssetName AM} 
+          {ckTrans: CKTrans FM Asset AM CK Configuration} 
+            {SPL: SPL Asset Configuration FM AM CK PL} : Prop :=
+    wfPL (gerPL fm2 am2 ck2) /\
+    wfCK_func fm2 am2 ck2 /\ forall an: AssetName,  ~(set_In an (dom_func am1)) /\ (~ set_In G (fst fm1)) /\
+    forall c: Configuration, forall expr, set_In expr (exps items) /\
+    satisfies expr c -> satisfies (NAME_FORMULA(G)) c.
+
+  Theorem addOptionalFeatureEqualProducts 
+    {Mp: Maps AssetName Asset AM}
+      {Ft: FormulaTheory Formula Name FM}
+        {FtM: FeatureModel FM Configuration} 
+          {AssetM: AssetMapping Asset AssetName AM} 
+            {ckTrans: CKTrans FM Asset AM CK Configuration} 
+              {SPL: SPL Asset Configuration FM AM CK PL} 
+                {FormT: FormulaTheory Formula Name FM} 
+                  {FMS: FeatureModelSemantics Formula FM Name }
+                    {FMR: FeatureModelRefinement Formula Name FM}:
+    forall pl (fm2: FM) (am2: AM) (ck2: CK) (F G: Name) (items:set Item) (pairs: AM),
+      wfCK_func (fst (fst pl)) (snd (fst pl)) (snd pl) /\
+        syntaxAddOptionalFeature (fst (fst pl)) (snd (fst pl)) (snd pl) fm2 am2 ck2 F G items pairs /\
+          conditionsAddOptionalFeature (fst (fst pl)) fm2 (snd (fst pl)) am2 pairs ck2 G items
+    ->
+      forall c, set_In c (semantics_func (fst (fst pl))) -> 
+        semantics_func_ (snd pl) (snd (fst pl)) c = semantics_func_ ck2 am2 c. 
+  Proof.
+  unfold syntaxAddOptionalFeature. unfold conditionsAddOptionalFeature.
+  simpl.  intros pl fm am ck F G items pairs. destruct pl. destruct p.
+  simpl. intuition.
+  specialize (H7 an). rewrite H6, H9. destruct f. destruct fm. 
+  simpl in H5, H2, H0, H6, H3, H1, H4, H8, H7. destruct H7. destruct H10. destruct G, F.
+  intuition.
+  Qed.
+
+
+  Theorem addOptionalFeature 
+    {Mp: Maps AssetName Asset AM}
+      {Ft: FormulaTheory Formula Name FM}
+        {FtM: FeatureModel FM Configuration} 
+          {AssetM: AssetMapping Asset AssetName AM} 
+            {ckTrans: CKTrans FM Asset AM CK Configuration} 
+              {SPL: SPL Asset Configuration FM AM CK PL} 
+                {FormT: FormulaTheory Formula Name FM} 
+                  {FMS: FeatureModelSemantics Formula FM Name }
+                    {FMR: FeatureModelRefinement Formula Name FM}:
+    forall (pl: PL) (fm2: FM) (am2: AM) (ck2: CK) (F G: Name) (items:set Item) (pairs: AM),
+      wfCK_func (getFM pl) (getAM pl) (getCK pl) /\
+        syntaxAddOptionalFeature (getFM pl) (getAM pl) (getCK pl) fm2 am2 ck2 F G items pairs  /\
+          conditionsAddOptionalFeature (getFM pl) fm2 (getAM pl) am2 pairs ck2 G items
+            -> plRefinement_func pl (gerPL fm2 am2 ck2) 
+              /\ wfCK_func fm2 am2 ck2 /\ wfPL (gerPL fm2 am2 ck2).
+  Proof. 
+  intros pl fm am ck F G items pairs. unfold syntaxAddOptionalFeature.
+  unfold conditionsAddOptionalFeature. intros. 
+  simpl. intuition. rewrite H6, H9. destruct gerPL. 
+  unfold plRefinement_func.  intros. exists c3. split.
+      +  destruct gerPL. unfold getFM_func. simpl.  unfold getFM_func in H8. destruct pl in H8. 
+        simpl in H8. destruct pls1. simpl. destruct p.
+        destruct pls2 in H8.  simpl in H8. destruct p.
+        simpl in H8. destruct f, f0. simpl. apply H8. 
+      +  specialize (H7 an). destruct H7. destruct H10. destruct G, F.
+        intuition.
+  Qed. 
+
+(*=================== ADD UNUSED ASSETS ===================*)
+
+Fixpoint assetsCK (items:set Item): set AssetName := 
+  match items with
+  | nil => nil
+  | x :: xs => x.(assets) ++ assetsCK xs
+  end.
+
+Definition Is_truePB (b:Prop) : bool :=
+    match b with
+      | True => true
+    end.
+
+
+Fixpoint remov (ls: set AssetName) am1: AM :=
+  match am1 with
+  | nil => nil
+  | x :: xs => if Is_truePB(set_In (fst x) (ls)) then remov ls xs else (x :: remov ls xs)
+  end.
+
+Definition syntaxAddUnusedAssets (am1 am2 pairs: AM) : Prop :=
+  am2 = app pairs (remov (dom_func pairs) am1).
+
+Definition conditionsAddUnusedAssets {Mp: Maps AssetName Asset AM} pairs ck: Prop :=
+  forall an, set_In an (dom_ pairs) -> (~ set_In an (assetsCK ck)).
+
+ Theorem addUnusedAssetsSameCK 
+  {Mp: Maps AssetName Asset AM}
+    {Ft: FormulaTheory Formula Name FM}
+      {FtM: FeatureModel FM Configuration} 
+        {AssetM: AssetMapping Asset AssetName AM} 
+          {ckTrans: CKTrans FM Asset AM CK Configuration} 
+            {SPL: SPL Asset Configuration FM AM CK PL}:
+  forall pl am2 pairs,
+    (
+      syntaxAddUnusedAssets (snd( fst pl)) am2 pairs /\
+        conditionsAddUnusedAssets pairs (snd pl)
+          -> forall (c: Configuration), set_In c (semantics_func (fst(fst pl)))
+            -> (semantics_func_ (snd pl) (snd( fst pl)) c) =
+              semantics_func_ (snd pl) am2 c).
+  Proof.
+  simpl. intuition. simpl. simpl in H0.
+  unfold syntaxAddUnusedAssets in H1.
+  unfold conditionsAddUnusedAssets in H2.
+  specialize (H2 an).  simpl in H1, H2, H0. rewrite H1.
+  simpl. 
+
+ (*
+  
+  destruct pl. destruct pls0. destruct p. destruct getFM.
+  destruct c0.
+  simpl. simpl in H1. unfold semantics_func in H1. simpl in H1. *)
+  Admitted.
+
+
+  Theorem addUnusedAssets
+  {Mp: Maps AssetName Asset AM}
+    {Ft: FormulaTheory Formula Name FM}
+      {FtM: FeatureModel FM Configuration}
+       {AssetM: AssetMapping Asset AssetName AM} 
+          {ckTrans: CKTrans FM Asset AM CK Configuration} 
+            {SPL: SPL Asset Configuration FM AM CK PL}:
+    forall pl am2 pairs,
+      (
+        syntaxAddUnusedAssets (getAM pl) am2 pairs /\
+        conditionsAddUnusedAssets pairs (getCK pl)
+      ->
+        strongerPLrefinement_func pl (gerPL (getFM pl) am2 (getCK pl)) 
+          /\ wfPL (gerPL (getFM pl) am2 (getCK pl))). 
+  Proof.
+   intros. destruct H0. unfold syntaxAddUnusedAssets in H0. 
+unfold conditionsAddUnusedAssets in H1.
+  specialize (H1 an). intuition.
+  - unfold strongerPLrefinement_func. intros. split.
+    + unfold getFM_func. simpl.  unfold getFM_func in H2. destruct pl in H2.
+        simpl in H2. destruct gerPL. destruct pls1. simpl. destruct p.
+        simpl in H2.  destruct pls0 in H2. simpl in H2. destruct p.
+        simpl in H2. destruct f, f0. simpl. apply H2.
+    + destruct gerPL. unfold getCK_func. unfold getAM_func. simpl.
+      induction pl, pls0. simpl. induction pls1. simpl. simpl in H0. admit.
+  - intuition. destruct gerPL. Search dom_.
+Admitted.
+
+(*================== REMOVE UNUSED ASSETS =======================*)
+
+  Theorem removeUnusedAssetsSameEvalCK  {Mp: Maps AssetName Asset AM}
+     {Ft: FormulaTheory Formula Name FM}
+      {FtM: FeatureModel FM Configuration} {AssetM: AssetMapping Asset AssetName AM} 
+          {ckTrans: CKTrans FM Asset AM CK Configuration} 
+            {SPL: SPL Asset Configuration FM AM CK PL}:
+    forall (pl: PL) am2 pairs,
+    (
+      syntaxAddUnusedAssets am2 (getAM pl) pairs /\
+      conditionsAddUnusedAssets pairs (getCK pl)
+      -> forall c, set_In c (semantics (getFM pl)) ->
+       (semantics_func_ (getCK pl) (getAM pl) c) =  semantics_func_ (getCK pl) am2 c). 
+  Proof.
+  unfold syntaxAddUnusedAssets. 
+  unfold conditionsAddUnusedAssets.
+  intuition.
+  specialize (H2 an). 
+  Admitted.
+
+
+  Theorem removeUnusedAssets{Mp: Maps AssetName Asset AM}
+    {Ft: FormulaTheory Formula Name FM}
+      {FtM: FeatureModel FM Configuration} {AssetM: AssetMapping Asset AssetName AM} 
+          {ckTrans: CKTrans FM Asset AM CK Configuration} 
+            {SPL: SPL Asset Configuration FM AM CK PL}:
+    forall pl am2 pairs,
+      (
+        syntaxAddUnusedAssets am2 (getAM pl) pairs /\
+        conditionsAddUnusedAssets pairs (getCK pl)
+      ->
+        strongerPLrefinement_func pl (gerPL (getFM pl) am2 (getCK pl)) /\ wfPL (gerPL (getFM pl) am2 (getCK pl))). 
+  Proof.
+  intros. destruct H0. unfold syntaxAddUnusedAssets in H0. 
+unfold conditionsAddUnusedAssets in H1.
+  specialize (H1 an). intuition.
+  - unfold strongerPLrefinement_func. intros. split.
+    + unfold getFM_func. simpl.  unfold getFM_func in H2. destruct pl in H2.
+        simpl in H2. destruct gerPL. destruct pls1. simpl. destruct p.
+        simpl in H2.  destruct pls0 in H2. simpl in H2. destruct p.
+        simpl in H2. destruct f, f0. simpl. apply H2.
+    + destruct gerPL. unfold getCK_func. unfold getAM_func. simpl.
+      induction pl, pls0. simpl. induction pls1. simpl. simpl in H0. intuition.
+
+  Admitted.
+
+End SpecificSPL.
+
