ck_comp.v
@@ -1,0 +1,190 @@
+Module CKComp.
+
+Require Export name form feature_model decidability feature_model_semantics formula_theory maps
+               feature_model_refinement asset_mapping assets.
+Import Name Decidability Form FeatureModel FeatureModelSemantics 
+       FeatureModelRefinements AssetMapping Assets FormulaTheory Maps.
+
+
+ Record Item : Type := {
+  exp_: Formula;
+  assets_: set AssetName;
+}.
+
+  Definition CK: Type := set Item.
+
+
+  Variable am am1 am2: AM.
+  Variable  an an1 an2: AssetName.
+  Variable fm: WFM.
+  Variable exp: Formula.
+  Variable ck: CK. 
+  Variable item it: Item.
+  Variable items its1 its2: list Item.
+  Variable c c1 c2: Configuration.
+  Variable F G H opt: Name.
+
+  (* get Formula*)
+  Definition getExp it: Formula := it.(exp_).
+  
+  (* get set AssetName*)
+  Definition getRS (it: Item) : set AssetName := it.(assets_).
+
+   (* Get all Formulas*)
+  Fixpoint exps ck : set Formula :=
+    match ck with
+    | nil => nil
+    | x :: xs => set_union form_dec (set_add form_dec (x.(exp_)) nil) (exps xs)
+    end.
+
+  Axiom item_dec : forall x y:Item, {x = y} + {x <> y}.
+
+  Fixpoint SetCompAux ck c: set Item :=
+    match ck with
+      | nil => nil
+      | x :: xs => if Is_truePB (satisfies (getExp x) c) then
+                   x :: (SetCompAux xs c) else (SetCompAux xs c)
+    end.
+
+  Lemma lemmaSetComp: forall ck c,
+    SetCompAux ck c = set_inter item_dec ck (SetCompAux ck c).
+  Proof.
+  induction ck0.
+  - intros.
+    simpl. reflexivity.
+  - specialize (IHck0 c).
+    intro c. 
+  Admitted.
+
+   (*evaluates a CK against a product configuration and
+     yields only CK items evaluated as true *)
+  Definition evalCK ck c : set Item := SetCompAux ck c.
+
+  (*yields all asset names referenced in a given set of CK items*)
+
+  Fixpoint assetsCK items: set AssetName :=
+    match items with
+      | nil => nil
+      | x :: xs =>  (x.(assets_)) ++ (assetsCK xs)
+    end.
+
+  (*  % yields all asset names of a given CK *)
+  Definition imgCK ck: set AssetName:=
+    assetsCK ck.
+
+  (*yields only the asset names evaluated as true for a given product configuration*)
+  Definition eval ck c: set AssetName :=
+    assetsCK (evalCK ck c).
+
+  (*yields only the asset names evaluated as true for a given product configuration*)
+  Definition eval2 ck c: set AssetName :=
+    assetsCK (evalCK ck c).
+
+  Definition notshowupItem it an : Prop :=
+    ~ set_In an (it.(assets_)).
+  
+  Definition showupItem it an: Prop :=
+    set_In an (it.(assets_)).
+  
+  Variable a: T.
+
+  (*yields the assets to build a product for a given product configuration 
+   sCK : [ConfigKnowledge->[AM->[Configuration->finite_sets[Asset].finite_set]]] =*)
+  Definition semantics_ (ck: CK) (am: AM) (c: Configuration) : set Asset := maps a am (eval ck c).
+
+  Axiom as_dec : forall x y: Asset, {x = y} + {x <> y}.
+  Axiom an_dec : forall x y: AssetName, {x = y} + {x <> y}.
+  Axiom its_dec : forall x y: Item, {x = y} + {x <> y}.
+  Axiom ns_dec : forall x y: Name, {x = y} + {x <> y}.
+    
+   (* Evaluate union*)
+  Lemma evalUnion: forall items its1 its2 c am,
+    items = set_union its_dec its1 its2
+      -> semantics_ items am c = set_union as_dec (semantics_ its1 am c) (semantics_ its2 am c).
+  Proof.
+  intuition.
+  rewrite H0. intuition.
+  Admitted. 
+
+  Definition wfCK (fm: WFM) am ck : Prop :=
+    wfFM fm /\ (forall c, set_In c (semantics fm) -> (set_diff an_dec (eval ck c) (dom am) = nil)) /\
+    (forall exp, set_In exp (exps ck) -> wt fm exp).
+
+  Definition wfCK2 (fm: FM) (am: AM) (ck:CK) : Prop :=
+    (forall item, set_In item ck -> (set_diff an_dec (item.(assets_)) (dom am) = nil)) /\
+    (forall exp, set_In exp (exps ck) -> wt fm exp).
+
+
+  (* esta vai ser nossa nocao de equivalencia*)
+  Definition ckEq (fm: WFM) am (ck1 ck2: CK) : Prop :=
+    forall c, set_In c (semantics fm) -> ((semantics_ ck1 am c) = (semantics_ ck2 am c)).
+
+  (*Equivalence properties - reflexive *)
+  Theorem eqReflexive:
+    forall fm am ck, ckEq fm am ck ck.
+  Proof.
+  intros. unfold ckEq.
+  intros. reflexivity.
+  Qed.
+
+  (*equivalence properties - symmetric*)
+  Theorem eqSymmetric:
+    forall fm am ck1 ck2, ckEq fm am ck1 ck2 -> ckEq fm am ck2 ck1.
+  Proof.
+  intros fm am ck1 ck2.
+  unfold ckEq. intros.
+  specialize (H0 c0). intuition.
+  Qed.
+
+  (* equivalence properties - transitive *)
+  Theorem eqTransitive:
+    forall fm am ck1 ck2 ck3,
+      ckEq fm am ck1 ck2 /\ ckEq fm am ck2 ck3 -> ckEq fm am ck1 ck3.  
+  Proof.
+  intros fm0 am0 ck1 ck2 ck3.
+  unfold ckEq. intros.
+  destruct H0. specialize (H0 c0). specialize (H2 c0).
+  intuition. rewrite H3, H0. reflexivity.
+  Qed.
+
+  (*esta vai ser nossa nocao de equivalencia *)
+  Definition ckEq2 ck1 ck2 : Prop :=
+    eval2 ck1 = eval2 ck2.
+
+  (*Equivalence properties - reflexive*)
+  Theorem eqReflexive2:
+    forall ck, ckEq2 ck ck.
+  Proof.
+  intro ck0. intuition.
+  Qed.
+
+  (*equivalence properties - symmetric*)
+  Theorem eqSymmetric2:
+    forall ck1 ck2,
+      ckEq2 ck1 ck2 -> ckEq2 ck2 ck1.
+  Proof.
+  intros. intuition.
+  Qed.
+
+  (*equivalence properties - transitive*)
+  Theorem eqTransitive2:
+    forall ck1 ck2 ck3,
+      ckEq2 ck1 ck2 /\ ckEq2 ck2 ck3 -> ckEq2 ck1 ck3.
+  Proof.
+  intros ck1 ck2 ck3. unfold ckEq2. intros.
+  destruct H0. rewrite H0, H1. reflexivity.
+  Qed. 
+
+
+End CKComp.
+  
+
+
+
+
+
+
+
+
+
+
