feature_model_refinement.v
@@ -1,0 +1,136 @@
+Module FeatureModelRefinements.
+
+Require Export form name decidability feature_model formula_theory feature_model_semantics.
+Import Name FormulaTheory Form Decidability FeatureModel FeatureModelSemantics.
+  Require Import Coq.Lists.ListSet.
+
+(*useful lemma*)
+
+Lemma wtFormAddNode: forall (abs con: FM) (n1 n2: Name),
+  wfTree(abs) /\ wfTree(con) /\
+    names_ (con) = set_add name_dec n2 (names_ (abs)) /\
+      set_In n1 (names_ (abs)) /\
+        (~set_In n2 (names_ (abs)))
+          -> (forall (f: Formula), wt abs f -> wt con f).
+Proof.
+  induction f. 
+  - intuition.
+  - intuition.
+  - destruct H. destruct H0. destruct H1. destruct H2.
+    intros. unfold not in H3.
+    unfold wt. unfold wt in H4. unfold names_ in H2.
+    unfold names_ in H3. unfold names_ in H1. rewrite H1. 
+    destruct n1, n2, n. intuition.
+  - intuition.
+  -  simpl. destruct H. destruct H0. destruct H1. destruct H2.
+    intros. unfold not in H3. destruct H4.
+    split. 
+    + apply IHf1. apply H4.
+    + apply IHf2. apply H5.
+  -  simpl. destruct H. destruct H0. destruct H1. destruct H2.
+    intros. unfold not in H3. destruct H4.
+    split. 
+    + apply IHf1. apply H4.
+    + apply IHf2. apply H5.
+Qed.
+
+(*===============  Add Mandatory Node ====================*)
+
+Definition addMandatoryNode (abs: WFM) (con: FM) (n1 n2: Name): Prop :=
+  names_ con = set_add name_dec n2 (names_ abs) /\
+      formulas con = set_union form_dec (app
+        ((IMPLIES_FORMULA (NAME_FORMULA(n2)) (NAME_FORMULA(n1)))::nil) 
+        ((IMPLIES_FORMULA (NAME_FORMULA(n1)) (NAME_FORMULA(n2)))::nil))
+          (formulas(abs)) /\  set_In n1 (names_ abs) /\ (~set_In n2 (names_ (abs))). 
+
+
+Theorem addMandatoryWF: forall (abs: WFM) (n1 n2: Name) (con:WFM),
+  addMandatoryNode abs con n1 n2 -> wfFM (con).
+Proof.
+  intros. 
+  unfold addMandatoryNode in H. destruct H. 
+  rewrite n1, n2 in H0. intuition.
+Qed.
+
+
+Theorem addMandatoryT: forall (abs: WFM) (n1 n2: Name),
+  exists (con: WFM), addMandatoryNode abs con n1 n2 ->
+    (forall (c: Configuration),
+      set_In c (semantics abs)
+        -> if Is_truePB(set_In n1 c) then (set_In (set_add name_dec n2 c) (semantics con))
+         else set_In c (semantics con)) /\
+           (forall (c: Configuration),
+              set_In c (semantics con)
+                -> if Is_truePB(set_In n2 c) then (set_In (set_remove name_dec n2 c) (semantics abs))
+                  else set_In c (semantics abs)) /\
+                    wfFM(con).
+Proof.
+  unfold addMandatoryNode. simpl. intros. exists abs.
+  intros. destruct H. destruct H0.  rewrite n1, n2 in H1.
+  intuition.
+Qed.
+
+Theorem addMandatoryTWF: forall (abs: WFM) (con: WFM) (n1 n2: Name),
+  addMandatoryNode abs con n1 n2 ->
+    (forall (c: Configuration),
+      set_In c (semantics abs)
+        -> if Is_truePB(set_In n1 c) then (set_In (set_add name_dec n2 c) (semantics con))
+         else set_In c (semantics con)) /\
+           (forall (c: Configuration),
+              set_In c (semantics con)
+                -> if Is_truePB(set_In n2 c) then (set_In (set_remove name_dec n2 c) (semantics abs))
+                  else set_In c (semantics abs)) /\
+                    wfFM(con).
+Proof.
+  simpl. intros. unfold addMandatoryNode in H. destruct H. destruct H0.
+  rewrite n1, n2 in H1. intuition.
+Qed.
+
+
+(*===================== Add Optional Node =====================*)
+
+
+Definition addOptionalNode (abs: WFM) (con: FM) (n1 n2: Name): Prop :=
+  names_ (con) = set_add name_dec n2 (names_ (abs)) /\ set_In n1 (names_ abs) /\
+     formulas (con) = set_add form_dec (IMPLIES_FORMULA (NAME_FORMULA(n2)) (NAME_FORMULA(n1)))
+          (formulas(abs)) /\ (~set_In n2 (names_ (abs))).  
+
+
+(*preserva a semantica estática*)
+Lemma wfPreservation: forall (abs: WFM) (con: WFM) (n1 n2: Name),
+  addOptionalNode abs con n1 n2 ->
+    wfFM (con).
+Proof.
+  intros. 
+  unfold addOptionalNode in H. destruct H. 
+  rewrite n1, n2 in H0. intuition.
+Qed.
+
+Theorem addNode: forall (abs: WFM) (con: WFM) (n1 n2: Name),
+  exists (con: WFM), (addOptionalNode abs con n1 n2 ->
+    refines abs con /\ wfFM con).
+Proof.
+  intros. 
+  exists abs. unfold addOptionalNode. intros. destruct H. 
+  rewrite n1, n2 in H0. intuition.
+Qed.
+
+Theorem addOptNode: forall (abs: WFM) (con: WFM) (n1 n2: Name),
+  addOptionalNode abs con n1 n2 -> 
+     refines abs con /\ wfFM con.
+Proof.
+  simpl. intros. unfold addOptionalNode in H. destruct H. destruct H0.
+  rewrite n2 in H1. rewrite n1 in H0. intuition.
+Qed.
+
+
+End FeatureModelRefinements.
+
+
+
+
+
+
+
+
+
