form.v
@@ -4,11 +4,11 @@ Require Export name.
 Import Name.
 
 Inductive Formula : Type :=
-  | TRUE_FORMULA : Formula
+  | TRUE_FORMULA  : Formula
   | FALSE_FORMULA : Formula
-  | NAME_FORMULA : Name -> Formula
-  | NOT_FORMULA : Formula -> Formula
-  | AND_FORMULA : Formula -> Formula -> Formula
+  | NAME_FORMULA  : Name -> Formula
+  | NOT_FORMULA   : Formula -> Formula
+  | AND_FORMULA   : Formula -> Formula -> Formula
   | IMPLIES_FORMULA : Formula -> Formula -> Formula.
 
 End Form.
